wip spilling

compiler/src/compiler/FlatImp.v
@@ -99,44 +99,53 @@ Section Syntax.
     | CondNez x => P x
     end.
 
-  Definition Forall_vars_stmt_gen{R: Type}(T: R)(and: R -> R -> R)(all: (varname -> R) -> list varname -> R)
-             (C: (varname -> R) -> bcond -> R)(P: varname -> R)(P_calls: varname -> R): stmt -> R :=
+  Definition Forall_vars_stmt_gen{R: Type}(T: R)(and: R -> R -> R)
+             (P_bcond: bcond -> R)
+             (P_vars: varname -> R)
+             (P_calls: list varname -> list varname -> R): stmt -> R :=
     fix rec s :=
       match s with
-      | SLoad _ x a _ => and (P x) (P a)
-      | SStore _ a x _ => and (P a) (P x)
-      | SInlinetable _ x _ i => and (P x) (P i)
-      | SStackalloc x n body => and (P x) (rec body)
-      | SLit x _ => P x
-      | SOp x _ y z => and (P x) (and (P y) (P z))
-      | SSet x y => and (P x) (P y)
-      | SIf c s1 s2 => and (C P c) (and (rec s1) (rec s2))
-      | SLoop s1 c s2 => and (C P c) (and (rec s1) (rec s2))
+      | SLoad _ x a _ => and (P_vars x) (P_vars a)
+      | SStore _ a x _ => and (P_vars a) (P_vars x)
+      | SInlinetable _ x _ i => and (P_vars x) (P_vars i)
+      | SStackalloc x n body => and (P_vars x) (rec body)
+      | SLit x _ => P_vars x
+      | SOp x _ y z => and (P_vars x) (and (P_vars y) (P_vars z))
+      | SSet x y => and (P_vars x) (P_vars y)
+      | SIf c s1 s2 => and (P_bcond c) (and (rec s1) (rec s2))
+      | SLoop s1 c s2 => and (P_bcond c) (and (rec s1) (rec s2))
       | SSeq s1 s2 => and (rec s1) (rec s2)
       | SSkip => T
-      | SCall binds _ args => and (all P_calls binds) (all P_calls args)
-      | SInteract binds _ args => and (all P_calls binds) (all P_calls args)
+      | SCall binds _ args => P_calls binds args
+      | SInteract binds _ args => P_calls binds args
       end.
 
-  Definition ForallVars_bcond(P: varname -> Prop)(cond: bcond): Prop :=
-    Eval unfold ForallVars_bcond_gen in ForallVars_bcond_gen and P cond.
+  Definition ForallVars_bcond(P_vars: varname -> Prop)(cond: bcond): Prop :=
+    Eval unfold ForallVars_bcond_gen in ForallVars_bcond_gen and P_vars cond.
 
-  Definition Forall_vars_stmt(P: varname -> Prop)(P_calls: varname -> Prop): stmt -> Prop :=
+  Definition Forall_vars_stmt(P_vars: varname -> Prop): stmt -> Prop :=
     Eval unfold Forall_vars_stmt_gen in
-      Forall_vars_stmt_gen True and (@Forall varname) ForallVars_bcond P P_calls.
+      Forall_vars_stmt_gen True and (ForallVars_bcond P_vars) P_vars
+                           (fun binds args => (List.length binds <= 8)%nat /\
+                                              (List.length args <= 8)%nat /\
+                                              Forall P_vars binds /\
+                                              Forall P_vars args).
 
-  Definition forallbVars_bcond(P: varname -> bool)(cond: bcond): bool :=
-    Eval unfold ForallVars_bcond_gen in ForallVars_bcond_gen andb P cond.
+  Definition forallbVars_bcond(P_vars: varname -> bool)(cond: bcond): bool :=
+    Eval unfold ForallVars_bcond_gen in ForallVars_bcond_gen andb P_vars cond.
 
-  Definition forallb_vars_stmt(P: varname -> bool)(P_calls: varname -> bool): stmt -> bool :=
+  Definition forallb_vars_stmt(P_vars: varname -> bool): stmt -> bool :=
     Eval unfold Forall_vars_stmt_gen in
-      Forall_vars_stmt_gen true andb (@forallb varname) forallbVars_bcond P P_calls.
+      Forall_vars_stmt_gen true andb (forallbVars_bcond P_vars) P_vars
+                           (fun binds args => (List.length binds <=? 8)%nat &&
+                                              (List.length args <=? 8)%nat &&
+                                              forallb P_vars binds &&
+                                              forallb P_vars args).
 
   Lemma forallb_vars_stmt_correct
-        (P: varname -> Prop)(p: varname -> bool)(P_calls: varname -> Prop)(p_calls: varname -> bool)
-        (p_correct: forall x, p x = true <-> P x)
-        (p_calls_correct: forall x, p_calls x = true <-> P_calls x):
-    forall s, forallb_vars_stmt p p_calls s = true <-> Forall_vars_stmt P P_calls s.
+        (P: varname -> Prop)(p: varname -> bool)
+        (p_correct: forall x, p x = true <-> P x):
+    forall s, forallb_vars_stmt p s = true <-> Forall_vars_stmt P s.
   Proof.
     assert (p_correct_fw: forall x, p x = true -> P x). {
       intros. eapply p_correct. assumption.
@@ -144,21 +153,17 @@ Section Syntax.
     assert (p_correct_bw: forall x, P x -> p x = true). {
       intros. eapply p_correct. assumption.
     }
-    assert (p_calls_correct_fw: forall x, p_calls x = true -> P_calls x). {
-      intros. eapply p_calls_correct. assumption.
-    }
-    assert (p_calls_correct_bw: forall x, P_calls x -> p_calls x = true). {
-      intros. eapply p_calls_correct. assumption.
-    }
-    clear p_correct p_calls_correct.
+    clear p_correct.
     induction s; split; simpl; intros; unfold ForallVars_bcond, forallbVars_bcond in *;
       repeat match goal with
              | c: bcond |- _ => destruct c
              | H: andb _ _ = true |- _ => eapply Bool.andb_true_iff in H
+             | H: (_ <=? _)%nat = true |- _ => eapply Nat.leb_le in H
              | H: _ /\ _ |- _ => destruct H
              | H: _ <-> _ |- _ => destruct H
              | |- andb _ _ = true => apply Bool.andb_true_iff
              | |- _ /\ _ => split
+             | |- (_ <=? _)%nat = true => eapply Nat.leb_le
              end;
       eauto using List.Forall_to_forallb, List.forallb_to_Forall.
   Qed.
@@ -170,21 +175,12 @@ Section Syntax.
     intros. destruct s; simpl in *; intuition eauto.
   Qed.
 
-  Lemma Forall_vars_stmt_impl: forall (P Q P_calls Q_calls: varname -> Prop),
+  Lemma Forall_vars_stmt_impl: forall (P Q: varname -> Prop),
       (forall x, P x -> Q x) ->
-      (forall x, P_calls x -> Q_calls x) ->
-      forall s, Forall_vars_stmt P P_calls s -> Forall_vars_stmt Q Q_calls s.
+      forall s, Forall_vars_stmt P s -> Forall_vars_stmt Q s.
   Proof.
     induction s; intros; simpl in *; intuition eauto using ForallVars_bcond_impl, Forall_impl.
   Qed.
-
-  Definition ForallVars_stmt P := Forall_vars_stmt P P.
-
-  Lemma ForallVars_stmt_impl: forall (P Q: varname -> Prop),
-      (forall x, P x -> Q x) ->
-      forall s, ForallVars_stmt P s -> ForallVars_stmt Q s.
-  Proof. unfold ForallVars_stmt. eauto using Forall_vars_stmt_impl. Qed.
-
 End Syntax.
 
 Arguments bcond: clear implicits.
